\documentclass[11pt]{article}
\usepackage{amsmath}
\begin{document}
\subsection*{1.}
\textbf{a.}The impulse response of the system $y(t) = x(t) + \alpha y(t - T)$  is simply:
\[h(t) = \sum_{k = 0}^\infty \alpha^k \delta(t - kT)  \]
\textbf{b.}
The system is BIBO stable if $\int_infty^\infty |h(t)|dt$ is bound. In our case we get that this integral is equal:
\[\int_\infty^\infty |\sum_{k = 0}^\infty \alpha^k \delta(t - kT)| dt\]
if alpha is positive we get that:
\[
\sum_{k = 0}^\infty \int_0^\infty \alpha^k \delta(t - kT)dt  = 
\sum_{k = 0}^\infty \alpha^k
\]
Which is bound if $\alpha < 1$ and unbound otherwise.
Hence, if $0 \leq \alpha < 1$ the system is BIBO stable, and it is unstable otherwise.\\
\textbf{c.}
An LTI system that would invert $h(t) = \sum_{k = 0}^\infty \alpha^k \delta(t - kT)$ is 
$\boxed{h_1(t) = \delta(t) - \alpha \delta(t - T)}$
We can show this by looking at the properties of the convolution.
\[y(t) = x(t) * h(t) \rightarrow h_1(t) * y(t) = h_1(t) * (x(t) * h(t)) = (h_1(t) * h(t)) * x(t)\]
Therefore, if $(h_1(t) * h(t)) = \delta(t)$ (which is trivial) we get that 
\[ h_1(t) * y(t)  = x(t)\]

\subsection*{2.}
\textbf{a.}
\textbf{ADD Diagram}\\
\textbf{b.}
\[\ddot{y}(t) + 300\dot{y}(t) + 2 \times 10^4 y(t) = 10^3 \dot{x}(t) \]
Since $e^{jwt}$ is an eigenfunction for the above LTI system, we get that
$y(t) = A_w e^{jwt}$, $\dot{y}(t) = A_w (jw) e^{jwt}$, $\ddot{y}(t) = A_w (wj)^2 e^{jwt}$
, and $\dot{x}(t) = (jw) e^{jwt}$ Substituting all of these into the equation yields:
\begin{align*}
A_w (jw)^2 e^{jwt} + A_w 300 (jw) e^{jwt} + A_w 2 \times 10^4 e^{jwt} = 10^3 e^{jwt} \rightarrow\\
e^{jwt} A_w ( (jw)^2 + 300(jw) + 10^4 ) = e^{jwt} 10^3 \rightarrow \\
A_w = \frac{10^3}{-w^2 + 10^4 + 300 w j}  = 
\boxed{\frac{10^3 (-w^2 + 10^4 - 300wj)}{ (-w^2 + 10^4)^2 + (300 w)^2}}
\end{align*}
\subsection*{3.}
\textbf{a.}
\textbf{ADD Diagram}\\
\textbf{b.}
\[y[n] + 300 y[n - 1] + 1700 y[n - 2] = x[n] + 20x[n-1]\]
Since $e^{jwn}$ is an eigenfunction for the above LTI system, we get that
$y[n] = A_w e^{jwt}$, $y[n - 1] = A_w e^{jwn} e^{-jw}$, $y[n - 2] = A_w  e^{jwn} e^{-2jw}$
,and $x[n] = e^{jwn}$ Substituting all of these into the equation yields:
\begin{align*}
A_w e^{jwt} + A_w e^{jwt}300  e^{-jw} + A_w e^{jwt} 1700 e{-2jw} =e^{jwt} + e^{jwt} 20 e^{-jw}= \\
A_w e^{jwt}(1 +  1300  e^{-jw} + 1700 e{-2jw}) =e^{jwt}(1 + 20e^{-jw}) \rightarrow \\
\boxed{A_w = \frac{(1 + 20e^{-jw})}{(1 +  1300  e^{-jw} + 1700 e{-2jw})}}
\end{align*}
\subsection*{4.}
\textbf{a.}
\textbf{b.}
\textbf{c.}
\subsection*{5.}
\textbf{a.}
\textbf{b.}
\subsection*{6.}
\textbf{a.}
\textbf{b.}
\textbf{c.}
\textbf{d.}
\end{document}


















